Auto/Embedding/LamChecker.lean
@@ -1,0 +1,14 @@
+import Auto.Embedding.LamConv
+import Auto.Lib.BinTree
+
+namespace Auto.Embedding.Lam
+
+structure TTable where
+  valid : Auto.BinTree (List LamSort × LamTerm)
+  wf    : Auto.BinTree (List LamSort × LamTerm × LamSort)
+
+inductive ChkStep where
+  | valid_of_interp (lctx : List LamSort) (t : LamTerm) (dest : Nat) : ChkStep
+  | wf_of_check (lctx : List LamSort) (t : LamTerm) (dest : Nat) : ChkStep
+
+end Auto.Embedding.Lam
